theories/Logic/inverse_dem_2.v
@@ -146,8 +146,8 @@ Definition demorgan2_sub_formula (A E F : formula) (S : subst_ind) : formula :=
         A
         (demorgan2_sub_formula D E F S_D)
         n d alpha
-        (fun (n : nat) =>
-            demorgan2_sub_ptree_fit (g n) E F (lor_ind (non_target A) S_D))
+        (fun (t : c_term) =>
+            demorgan2_sub_ptree_fit (g t) E F (lor_ind (non_target A) S_D))
   
   | cut_ca C0 A d1 d2 alpha1 alpha2 P1 P2, _ =>
       cut_ca
@@ -657,18 +657,18 @@ Definition demorgan2_sub_formula (A E F : formula) (S : subst_ind) : formula :=
   
   - simpl. destruct S; apply H.
   
-  - simpl. destruct S; try apply H. inversion H as [[[[H0 H1] H2] H3] H4].
-    destruct S1; inversion Hs; rewrite H6; simpl.
+  - simpl. destruct S; try apply H. inversion H as [[[H0 H1] H2] H3].
+    destruct S1; inversion Hs; rewrite H5; simpl.
     + repeat split; auto.
       * rewrite demorgan2_ptree_formula_true, demorgan2_ptree_formula; auto.
         { rewrite H0. unfold demorgan2_sub_formula.
           { rewrite formula_sub_ind_lor. simpl.
-            { destruct (eq_f (substitution f n t)); auto. }
-            { simpl. apply H6. } } }
-        { rewrite H0. simpl. apply H6. }
+            { destruct (eq_f (substitution f n (projT1 c))); auto. }
+            { simpl. apply H5. } } }
+        { rewrite H0. simpl. apply H5. }
       * rewrite demorgan2_ptree_formula_true.
-        { apply IHP; auto. rewrite H0. simpl. apply H6. }
-        { rewrite H0. simpl. apply H6. }
+        { apply IHP; auto. rewrite H0. simpl. apply H5. }
+        { rewrite H0. simpl. apply H5. }
       * rewrite demorgan2_ptree_formula_true.
         { rewrite demorgan2_ptree_deg; auto. }
         { rewrite H0. simpl. auto. }
@@ -679,12 +679,12 @@ Definition demorgan2_sub_formula (A E F : formula) (S : subst_ind) : formula :=
       * rewrite demorgan2_ptree_formula_true, demorgan2_ptree_formula; auto.
         { rewrite H0. unfold demorgan2_sub_formula.
           { rewrite formula_sub_ind_lor. simpl.
-            { destruct (eq_f (substitution f n t)); auto. }
-            { simpl. apply H6. } } }
-        { rewrite H0. simpl. apply H6. }
+            { destruct (eq_f (substitution f n (projT1 c))); auto. }
+            { simpl. apply H5. } } }
+        { rewrite H0. simpl. apply H5. }
       * rewrite demorgan2_ptree_formula_true.
-        { apply IHP; auto. rewrite H0. simpl. apply H6. }
-        { rewrite H0. simpl. apply H6. }
+        { apply IHP; auto. rewrite H0. simpl. apply H5. }
+        { rewrite H0. simpl. apply H5. }
       * rewrite demorgan2_ptree_formula_true.
         { rewrite demorgan2_ptree_deg; auto. }
         { rewrite H0. simpl. auto. }
@@ -696,53 +696,53 @@ Definition demorgan2_sub_formula (A E F : formula) (S : subst_ind) : formula :=
   
   - rename H into H0. rename X into H. rename Hs into H1.
     simpl. destruct S; try apply H0. destruct S1; inversion H1.
-    + rewrite H3. simpl. intros. destruct (valid_w_rule_ad _ _ _ _ _ _ H0 m)  as [[[H4 H5] H6] H7].
+    + rewrite H3. simpl. intros. destruct (valid_w_rule_ad _ _ _ _ _ _ H0 t)  as [[[H4 H5] H6] H7].
       repeat split.
       * rewrite demorgan2_ptree_formula_true, demorgan2_ptree_formula; auto.
         { rewrite H4. unfold demorgan2_sub_formula. rewrite formula_sub_ind_lor.
-          { rewrite (non_target_term_sub f n (represent m)).
+          { rewrite (non_target_term_sub f n (projT1 t)).
             rewrite non_target_sub. auto. }
-          { rewrite (non_target_term_sub f n (represent m)).
+          { rewrite (non_target_term_sub f n (projT1 t)).
             rewrite non_target_fit. apply H3. } }
-        { rewrite H4. simpl. rewrite (non_target_term_sub f n (represent m)).
+        { rewrite H4. simpl. rewrite (non_target_term_sub f n (projT1 t)).
           rewrite non_target_fit. apply H3. }
       * rewrite demorgan2_ptree_formula_true.
         { apply H. apply H5. rewrite H4. simpl.
-          rewrite (non_target_term_sub f n (represent m)).
+          rewrite (non_target_term_sub f n (projT1 t)).
           rewrite non_target_fit. apply H3. }
-        { rewrite H4. simpl. rewrite (non_target_term_sub f n (represent m)).
+        { rewrite H4. simpl. rewrite (non_target_term_sub f n (projT1 t)).
           rewrite non_target_fit. apply H3. }
       * rewrite demorgan2_ptree_formula_true.
         { rewrite demorgan2_ptree_deg; auto. }
-        { rewrite H4. simpl. rewrite (non_target_term_sub f n (represent m)).
+        { rewrite H4. simpl. rewrite (non_target_term_sub f n (projT1 t)).
           rewrite non_target_fit. rewrite H3. auto. }
       * rewrite demorgan2_ptree_formula_true.
         { rewrite demorgan2_ptree_ord; auto. }
-        { rewrite H4. simpl. rewrite (non_target_term_sub f n (represent m)).
+        { rewrite H4. simpl. rewrite (non_target_term_sub f n (projT1 t)).
           rewrite non_target_fit. rewrite H3. auto. }
-    + rewrite H3. simpl. intros. destruct (valid_w_rule_ad _ _ _ _ _ _ H0 m) as [[[H4 H5] H6] H7].
+    + rewrite H3. simpl. intros. destruct (valid_w_rule_ad _ _ _ _ _ _ H0 t) as [[[H4 H5] H6] H7].
       repeat split.
       * rewrite demorgan2_ptree_formula_true, demorgan2_ptree_formula; auto.
         { rewrite H4. unfold demorgan2_sub_formula. rewrite formula_sub_ind_lor.
-          { rewrite (non_target_term_sub f n (represent m)).
+          { rewrite (non_target_term_sub f n (projT1 t)).
             rewrite non_target_sub. auto. }
-          { rewrite (non_target_term_sub f n (represent m)).
+          { rewrite (non_target_term_sub f n (projT1 t)).
             rewrite non_target_fit. apply H3. } }
-        { rewrite H4. simpl. rewrite (non_target_term_sub f n (represent m)).
+        { rewrite H4. simpl. rewrite (non_target_term_sub f n (projT1 t)).
           rewrite non_target_fit. apply H3. }
       * rewrite demorgan2_ptree_formula_true.
         { apply H. apply H5. rewrite H4. simpl.
-          rewrite (non_target_term_sub f n (represent m)).
+          rewrite (non_target_term_sub f n (projT1 t)).
           rewrite non_target_fit. apply H3. }
-        { rewrite H4. simpl. rewrite (non_target_term_sub f n (represent m)).
+        { rewrite H4. simpl. rewrite (non_target_term_sub f n (projT1 t)).
           rewrite non_target_fit. apply H3. }
       * rewrite demorgan2_ptree_formula_true.
         { rewrite demorgan2_ptree_deg; auto. }
-        { rewrite H4. simpl. rewrite (non_target_term_sub f n (represent m)).
+        { rewrite H4. simpl. rewrite (non_target_term_sub f n (projT1 t)).
           rewrite non_target_fit. rewrite H3. auto. }
       * rewrite demorgan2_ptree_formula_true.
         { rewrite demorgan2_ptree_ord; auto. }
-        { rewrite H4. simpl. rewrite (non_target_term_sub f n (represent m)).
+        { rewrite H4. simpl. rewrite (non_target_term_sub f n (projT1 t)).
           rewrite non_target_fit. rewrite H3. auto. }
   - clear IHP2. simpl. destruct (subst_ind_fit f S) eqn:Heq; try apply H. simpl.
     inversion H as [[[[[[[H1 H2] H3] H4] H5] H6] H7] H8].
