theories/Logic/inverse_neg.v
@@ -127,8 +127,8 @@ match P, S with
       (dub_neg_sub_formula D E S_D)
       n
       d alpha
-      (fun (n : nat) =>
-          dub_neg_sub_ptree_fit (g n) E (lor_ind (non_target A) S_D))
+      (fun (t : c_term) =>
+          dub_neg_sub_ptree_fit (g t) E (lor_ind (non_target A) S_D))
 
 | cut_ca C0 A d1 d2 alpha1 alpha2 P1 P2, _ =>
     cut_ca
@@ -671,18 +671,18 @@ induction P; try intros H S Hs.
 
 - simpl. destruct S; apply H.
 
-- simpl. destruct S; try apply H. inversion H as [[[[H0 H1] H2] H3] H4].
-  destruct S1; inversion Hs; rewrite H6; simpl.
+- simpl. destruct S; try apply H. inversion H as [[[H0 H1] H2] H3].
+  destruct S1; inversion Hs; rewrite H5; simpl.
   + repeat split; auto.
     * rewrite dub_neg_ptree_formula_true, dub_neg_ptree_formula; auto.
       { rewrite H0. unfold dub_neg_sub_formula.
         { rewrite formula_sub_ind_lor. simpl.
-          { destruct (eq_f (substitution f n t)); auto. }
-          { simpl. apply H6. } } }
-      { rewrite H0. simpl. apply H6. }
+          { destruct (eq_f (substitution f n (projT1 c))); auto. }
+          { simpl. apply H5. } } }
+      { rewrite H0. simpl. apply H5. }
     * rewrite dub_neg_ptree_formula_true.
-      { apply IHP; auto. rewrite H0. simpl. apply H6. }
-      { rewrite H0. simpl. apply H6. }
+      { apply IHP; auto. rewrite H0. simpl. apply H5. }
+      { rewrite H0. simpl. apply H5. }
     * rewrite dub_neg_ptree_formula_true.
       { rewrite dub_neg_ptree_deg; auto. }
       { rewrite H0. simpl. auto. }
@@ -693,12 +693,12 @@ induction P; try intros H S Hs.
     * rewrite dub_neg_ptree_formula_true, dub_neg_ptree_formula; auto.
       { rewrite H0. unfold dub_neg_sub_formula.
         { rewrite formula_sub_ind_lor. simpl.
-          { destruct (eq_f (substitution f n t)); auto. }
-          { simpl. apply H6. } } }
-      { rewrite H0. simpl. apply H6. }
+          { destruct (eq_f (substitution f n (projT1 c))); auto. }
+          { simpl. apply H5. } } }
+      { rewrite H0. simpl. apply H5. }
     * rewrite dub_neg_ptree_formula_true.
-      { apply IHP; auto. rewrite H0. simpl. apply H6. }
-      { rewrite H0. simpl. apply H6. }
+      { apply IHP; auto. rewrite H0. simpl. apply H5. }
+      { rewrite H0. simpl. apply H5. }
     * rewrite dub_neg_ptree_formula_true.
       { rewrite dub_neg_ptree_deg; auto. }
       { rewrite H0. simpl. auto. }
@@ -710,53 +710,53 @@ induction P; try intros H S Hs.
 
 - rename H into H0. rename X into H. rename Hs into H1.
   simpl. destruct S; try apply H0. destruct S1; inversion H1.
-  + rewrite H3. simpl. intros. destruct (valid_w_rule_ad _ _ _ _ _ _ H0 m) as [[[H4 H5] H6] H7].
+  + rewrite H3. simpl. intros. destruct (valid_w_rule_ad _ _ _ _ _ _ H0 t) as [[[H4 H5] H6] H7].
     repeat split.
     * rewrite dub_neg_ptree_formula_true, dub_neg_ptree_formula; auto.
       { rewrite H4. unfold dub_neg_sub_formula.
         rewrite formula_sub_ind_lor;
-        rewrite (non_target_term_sub f n (represent m)).
+        rewrite (non_target_term_sub f n (projT1 t)).
         { rewrite non_target_sub. auto. }
         { rewrite non_target_fit. apply H3. } }
-      { rewrite H4. simpl. rewrite (non_target_term_sub f n (represent m)).
+      { rewrite H4. simpl. rewrite (non_target_term_sub f n (projT1 t)).
         rewrite non_target_fit. apply H3. }
     * rewrite dub_neg_ptree_formula_true.
       { apply H. apply H5. rewrite H4. simpl.
-        rewrite (non_target_term_sub f n (represent m)).
+        rewrite (non_target_term_sub f n (projT1 t)).
         rewrite non_target_fit. apply H3. }
-      { rewrite H4. simpl. rewrite (non_target_term_sub f n (represent m)).
+      { rewrite H4. simpl. rewrite (non_target_term_sub f n (projT1 t)).
         rewrite non_target_fit. apply H3. }
     * rewrite dub_neg_ptree_formula_true.
       { rewrite dub_neg_ptree_deg; auto. }
-      { rewrite H4. simpl. rewrite (non_target_term_sub f n (represent m)).
+      { rewrite H4. simpl. rewrite (non_target_term_sub f n (projT1 t)).
         rewrite non_target_fit. rewrite H3. auto. }
     * rewrite dub_neg_ptree_formula_true.
       { rewrite dub_neg_ptree_ord; auto. }
-      { rewrite H4. simpl. rewrite (non_target_term_sub f n (represent m)).
+      { rewrite H4. simpl. rewrite (non_target_term_sub f n (projT1 t)).
         rewrite non_target_fit. rewrite H3. auto. }
-  + rewrite H3. simpl. intros. destruct (valid_w_rule_ad _ _ _ _ _ _ H0 m) as [[[H4 H5] H6] H7].
+  + rewrite H3. simpl. intros. destruct (valid_w_rule_ad _ _ _ _ _ _ H0 t) as [[[H4 H5] H6] H7].
     repeat split.
     * rewrite dub_neg_ptree_formula_true, dub_neg_ptree_formula; auto.
       { rewrite H4. unfold dub_neg_sub_formula. rewrite formula_sub_ind_lor.
-        { rewrite (non_target_term_sub f n (represent m)).
+        { rewrite (non_target_term_sub f n (projT1 t)).
           rewrite non_target_sub. auto. }
-        { rewrite (non_target_term_sub f n (represent m)).
+        { rewrite (non_target_term_sub f n (projT1 t)).
           rewrite non_target_fit. apply H3. } }
-      { rewrite H4. simpl. rewrite (non_target_term_sub f n (represent m)).
+      { rewrite H4. simpl. rewrite (non_target_term_sub f n (projT1 t)).
         rewrite non_target_fit. apply H3. }
     * rewrite dub_neg_ptree_formula_true.
       { apply H. apply H5. rewrite H4. simpl.
-        rewrite (non_target_term_sub f n (represent m)).
+        rewrite (non_target_term_sub f n (projT1 t)).
         rewrite non_target_fit. apply H3. }
-      { rewrite H4. simpl. rewrite (non_target_term_sub f n (represent m)).
+      { rewrite H4. simpl. rewrite (non_target_term_sub f n (projT1 t)).
         rewrite non_target_fit. apply H3. }
     * rewrite dub_neg_ptree_formula_true.
       { rewrite dub_neg_ptree_deg; auto. }
-      { rewrite H4. simpl. rewrite (non_target_term_sub f n (represent m)).
+      { rewrite H4. simpl. rewrite (non_target_term_sub f n (projT1 t)).
         rewrite non_target_fit. rewrite H3. auto. }
     * rewrite dub_neg_ptree_formula_true.
       { rewrite dub_neg_ptree_ord; auto. }
-      { rewrite H4. simpl. rewrite (non_target_term_sub f n (represent m)).
+      { rewrite H4. simpl. rewrite (non_target_term_sub f n (projT1 t)).
         rewrite non_target_fit. rewrite H3. auto. }
 - clear IHP2. simpl. destruct (subst_ind_fit f S) eqn:Heq; try apply H. simpl.
   inversion H as [[[[[[[H1 H2] H3] H4] H5] H6] H7] H8].
